compile record update

lang/Syntax.v
@@ -1,61 +1,131 @@
-From quartz Require VerilogSyntax.
-
-From stdpp Require Import base bitvector vector.
-From Stdlib Require Import 
-  List 
-  NArith 
-  Program.Equality 
-  String.
+From Stdlib Require Import BinInt Bits Vector.
+From Stdlib Require Import String List.
 Import ListNotations.
-
-Set Implicit Arguments.
-Set Asymmetric Patterns.
+Local Coercion Zmod.unsigned : Zmod >-> Z.
 
 Open Scope Z_scope.
 
 Module type.
+  Local Set Boolean Equality Schemes.
   Inductive type :=
   | Bool
-  | Bits (sz: N)
-  | Pair (t1 t2: type) (* TODO: name hint for struct fields?*)
+  | Bits (sz: Z)
+  | Pair (_ _ : type)
+  | Struct (_ : list (string * type))
   | Array (t: type) (sz: nat).
-  
-  Fixpoint type_denote tau : Type :=
-    match tau with
+
+  Fixpoint interp t : Type :=
+    match t with
     | Bool => bool
-    | Bits sz => bv sz
-    | Pair t1 t2 => (type_denote t1) * (type_denote t2)
-    | Array ty n => vec (type_denote ty) n 
+    | Bits sz => bits sz
+    | Pair a b => interp a * interp b
+    | Struct nts => fold_right (fun nt T => interp (snd nt) * T)%type unit nts
+    | Array t n => Vector.t (interp t) n
     end.
+
+  Definition struct := list (string * type).
+  Definition Struct_ : struct -> type := Struct.
+  Coercion Struct_ : struct >-> type.
+
+  Coercion type.interp: type >-> Sortclass.
+
+  Section WithInhabited.
+  Context (inhabited : forall t : type, t).
+  Fixpoint inhabited_struct (s : struct) : s :=
+    match s with
+    | nil => tt
+    | cons (_, t) s => (inhabited t, inhabited_struct s)
+    end.
+  Context (t : type).
+  Fixpoint inhabited_array (n : nat) :=
+    match n return Vector.t t n with
+    | O => Vector.nil _
+    | S n => Vector.cons (type.interp t) (inhabited t) n (inhabited_array n)
+    end.
+  End WithInhabited.
+  Fixpoint inhabited (t : type) : t. refine
+    match t return t with
+    | Bool => false
+    | Bits sz => Zmod.zero
+    | Pair a b => (inhabited a, inhabited b)
+    | Struct s => inhabited_struct inhabited s
+    | Array t n => inhabited_array inhabited t n
+    end.
+  Qed.
+
+  Global Opaque inhabited inhabited_array inhabited_struct.
+
+  Fixpoint eq_dec (a b : type) : { a = b } + { a <> b }. refine
+    match a, b with
+    | Bool, Bool => left eq_refl
+    | Bits a, Bits b =>
+        match Z.eq_dec a b with left _ => left _ | right _ => right _ end
+    | Struct a, Struct b =>
+        match list_eq_dec (fun '(sa, a) '(sb, b) =>
+          match string_dec sa sb, eq_dec a b with left _, left _ => left _ | _, _ => right _ end
+        ) a b with | left _ => left _ | right _ => right _ end
+    | Pair a1 a2, Pair b1 b2 =>
+        match eq_dec a1 b1, eq_dec a2 b2 with | left _, left _ => left _ | _, _ => right _ end
+    | Array a n, Array b m =>
+        match eq_dec a b, PeanoNat.Nat.eq_dec n m with | left _, left _ => left _ | _, _ => right _ end
+    | _, _ => right _
+    end.
+  all : abstract congruence.
+  Defined.
 End type.
 
 Import type.
-Coercion type_denote: type >-> Sortclass.
-Notation Unit := (Bits 0).
-Notation unit_value := (bv_0 0).
+Notation Unit := (Bits 0) (only parsing).
+Notation unit_value := (bits.of_Z _ 0) (only parsing).
 
-(* TODO: structs & array ops ; zeroExtend *)
+Module struct.
+  Notation struct := type.struct (only parsing).
+  Search NoDup bool.
+
+  Definition has (s : struct) (n : string) (t : type) : bool :=
+    existsb (fun nt => String.eqb (fst nt) n && type_beq (snd nt) t)%bool s.
+  Definition Has s n t := Bool.Is_true (has s n t).
+
+  Fixpoint get {s : struct} (n : string) (t : type) : s -> t :=
+    match s with | nil => fun _ => inhabited t | cons (nf, tf) s' =>
+    match String.eqb nf n with | false => fun s => @get _ n t (snd s) | true =>
+    match type.eq_dec tf t with | right _ => fun s => @get _ n t (snd s) | left pf =>
+    fun s => eq_rect tf type.interp (fst s) _ pf
+    end end end.
+
+  Fixpoint upd {s : struct} (n : string) (t : type) : s -> (t -> t) -> s :=
+    match s with | nil => fun s _ => s | cons (nf, tf) s' =>
+    match String.eqb nf n with | false => fun s v => (fst s, @upd s' n t (snd s) v) | true =>
+    match type.eq_dec t tf with | right _ => fun s v => (fst s, @upd s' n t (snd s) v) | left pf =>
+    fun s v => (eq_rect t (fun t => type.interp t -> type.interp t) v _ pf (fst s) , snd s)
+    end end end.
+
+  Definition put {s : struct} (n : string) (t : type) (sv : s) (v : t) :=
+    @upd s n t sv (fun _ => v).
+
+  Local Open Scope string_scope.
+  Example get_ab_b : @get [("a", Bits 7); ("b", Bool)] "b" Bool = fun r => fst (snd r).
+  Proof. cbv [get eq_dec eq_rect String.eqb Ascii.eqb Bool.eqb]. trivial. Qed.
+  Example get_ab_c : @get [("a", Bits 7); ("b", Bool)] "c" Bool = fun r => inhabited Bool.
+  Proof. cbv [get eq_dec eq_rect String.eqb Ascii.eqb Bool.eqb]. trivial. Qed.
+End struct.
+
 Module unop.
   Inductive unop : type -> type -> Type :=
   | Not {n} : unop (Bits n) (Bits n)
-  | Fst {a b: type} : unop (Pair a b) a
-  | Snd {a b: type} : unop (Pair a b) b.
+  .
 
-  Definition interp {a b} (op: unop a b) : type_denote a -> type_denote b :=
-    match op with
-    | Not _ => bv_not 
-    | Fst _ _ => fst 
-    | Snd _ _ => snd
-    end. 
+  Definition interp {a b} (op: unop a b) : type.interp a -> type.interp b :=
+    match op in unop a b return a -> b with
+    | Not => Zmod.not
+    end.
 End unop.
 Notation unop := unop.unop (only parsing).
 
 Module binop.
+  Inductive compare := cLt | cGt | cLe | cGe.
 
-  Inductive bits_comparison :=
-  | cLt | cGt | cLe | cGe.
-
-  Inductive binop : type -> type -> type -> Type := 
+  Inductive binop : type -> type -> type -> Type :=
   | Plus {n} : binop (Bits n) (Bits n) (Bits n)
   | And {n} : binop (Bits n) (Bits n) (Bits n)
   | Or {n} : binop (Bits n) (Bits n) (Bits n)
@@ -63,32 +133,24 @@ Module binop.
   | Lsr {n} : binop (Bits n) (Bits n) (Bits n)
   | Asr {n} : binop (Bits n) (Bits n) (Bits n)
   | EqBits {n} : binop (Bits n) (Bits n) Bool
-  | Compare (signed: bool) (c: bits_comparison) {n} : binop (Bits n) (Bits n) Bool
+  | Compare (signed: bool) (c: compare) {n} : binop (Bits n) (Bits n) Bool
   | MkPair {a b: type} : binop a b (Pair a b).
 
-  Definition interp {a b c} (op: binop a b c) 
-    : type_denote a -> type_denote b -> type_denote c :=
-    match op with
-    | Plus _ => bv_add
-    | And _ => bv_and
-    | Or _ => bv_or
-    | Lsl _ => bv_shiftl
-    | Lsr _ => bv_shiftr
-    | Asr _ => bv_ashiftr
-    | EqBits _ => fun b1 b2 => bool_decide (b1 = b2)
-    | Compare signed c _ => fun b1 b2 => 
-        match signed, c with
-        | true, cLt =>  bool_decide (bv_signed b1 < bv_signed b2)
-        | false, cLt => bool_decide (bv_unsigned b1 < bv_unsigned b2)
-        | true, cGt =>  bool_decide (bv_signed b1 > bv_signed b2)
-        | false, cGt => bool_decide (bv_unsigned b1 > bv_unsigned b2)
-        | true, cLe =>  bool_decide (bv_signed b1 <= bv_signed b2)
-        | false, cLe => bool_decide (bv_unsigned b1 <= bv_unsigned b2)
-        | true, cGe =>  bool_decide (bv_signed b1 >= bv_signed b2)
-        | false, cGe => bool_decide (bv_unsigned b1 >= bv_unsigned b2)
-        end
-    | MkPair _ _ => Datatypes.pair
-    end. 
+  Definition interp {a b c} (op: binop a b c) : a -> b -> c :=
+    match op in binop a b c return a -> b -> c with
+    | Plus => Zmod.add
+    | And => Zmod.and
+    | Or => Zmod.or
+    | Lsl => fun a b => Zmod.slu a b
+    | Lsr => fun a b => Zmod.sru a b
+    | Asr => fun a b => Zmod.srs a b
+    | EqBits => Zmod.eqb
+    | Compare signed c => fun a b =>
+        match c with cLt => Z.ltb | cGt => Z.gtb | cLe => Z.leb | cGe => Z.geb end
+        (if signed then Zmod.signed a else Zmod.unsigned a)
+        (if signed then Zmod.signed b else Zmod.unsigned b)
+    | MkPair => Datatypes.pair
+    end.
 End binop.
 Notation binop := binop.binop (only parsing).
 
@@ -97,72 +159,79 @@ Module typeWithHole.
   | HOLE
   | PairL (t1 : typeWithHole) (t2: type)
   | PairR (t1 : type) (t2: typeWithHole)
-  | Array (sz: nat) (idx: fin sz) (t: typeWithHole).
+  | Struct (l : struct) (n : string) (t : typeWithHole) (r : struct)
+  | Array (sz: nat) (t: typeWithHole).
 
   Fixpoint plug (C : typeWithHole) (t : type) : type :=
     match C with
     | HOLE => t
     | PairL t1 t2 => type.Pair (plug t1 t) t2
     | PairR t1 t2 => type.Pair t1 (plug t2 t)
-    | Array sz _ t' => type.Array (plug t' t) sz
+    | Struct l n C r => type.Struct (l ++ cons (n, plug C t) r)
+    | Array sz t' => type.Array (plug t' t) sz
     end.
 
-  Fixpoint fieldUpdate {C: typeWithHole.typeWithHole} {t: type} 
-    (r : type_denote (typeWithHole.plug C t)) (v : type_denote t) 
-    : (type_denote (typeWithHole.plug C t)) :=
-    match C return type_denote (typeWithHole.plug C t) -> (type_denote (typeWithHole.plug C t)) with
-    | typeWithHole.HOLE => fun r => v
-    | typeWithHole.PairL t1 t2 => fun r => (fieldUpdate r.1 v, r.2)
-    | typeWithHole.PairR t1 t2 => fun r => (r.1, fieldUpdate r.2 v)
-    | typeWithHole.Array sz idx t => fun r =>
-         Vector.replace r idx (fieldUpdate (r !!! idx) v)
-    end r.
+  Fixpoint indices (t : typeWithHole) : type :=
+    match t with
+    | HOLE => Unit
+    | PairL t _ | PairR _ t | Struct _ _ t _ => indices t
+    | Array sz t => Pair (Bits (Z.log2_up (Z.of_nat sz))) (indices t)
+    end.
 
-  Fixpoint getField {C: typeWithHole.typeWithHole} {t: type} 
-    (r : type_denote (typeWithHole.plug C t)) 
-    : type_denote t :=
-    match C return type_denote (typeWithHole.plug C t) -> (type_denote t) with
-    | typeWithHole.HOLE => fun r => r
-    | typeWithHole.PairL t1 _ => fun r => @getField t1 t r.1 
-    | typeWithHole.PairR _ t2 => fun r => @getField t2 t r.2
-    | typeWithHole.Array sz idx t' => fun r =>
-        @getField t' t (r!!! idx)                                      
-    end r.
+  Axiom Vector__get : forall {T n}, Vector.t T n -> bits (Z.log2_up (Z.of_nat n)) -> T.
+  Axiom Vector__mod : forall {T n}, Vector.t T n -> bits (Z.log2_up (Z.of_nat n)) -> (T -> T) -> Vector.t T n.
 
+  Fixpoint getField C : forall t, plug C t -> indices C -> t :=
+    match C with
+    | HOLE => fun t r i => r
+    | PairL a b => fun _ r i => getField a _ (fst r) i
+    | PairR a b => fun _ r i => getField b _ (snd r) i
+    | Struct _ n t _ => fun _ r i => getField t _ (struct.get n _ r) i
+    | Array sz t => fun _ r i => getField t _ (Vector__get r (fst i)) (snd i)
+    end.
+  Arguments getField {_ _}.
+
+  Fixpoint updField C : forall t, plug C t -> indices C -> (t -> t) -> plug C t :=
+    match C with
+    | HOLE => fun t r i f => f r
+    | PairL a b => fun _ r i v => (updField a _ (fst r) i v, snd r)
+    | PairR a b => fun _ r i v => (fst r, updField b _ (snd r) i v)
+    | Struct _ n t _ => fun _ r i v => struct.upd n _ r v
+    | Array sz t => fun _ r i v => Vector__mod r (fst i) (fun r => updField _ _ r (snd i) v)
+    end.
+  Arguments updField {_ _}.
 End typeWithHole.
+Notation typeWithHole :=typeWithHole.typeWithHole (only parsing).
+
+Coercion typeWithHole.plug : typeWithHole >-> Funclass.
+Coercion typeWithHole.indices : typeWithHole >-> type.
 
 Module expr.
   Section WithSubstitutionType.
     Context {var: type -> Type}.
-
-    (* TODO: value method call *)
-    Inductive expr : type -> Type := 
+    Inductive expr : type -> Type :=
     | Var {tx: type} (x: var tx) : expr tx
-    | Const {tc: type} (c: type_denote tc) : expr tc
+    | Const {tc: type} (c: type.interp tc) : expr tc
     | Unop {t1 tR: type} (op: unop t1 tR) (e1: expr t1) : expr tR
     | Binop {t1 t2 tR: type} (op: binop t1 t2 tR) (e1: expr t1) (e2: expr t2) : expr tR
-    | ITE {k: type} (cond: expr Bool) (tbranch fbranch: expr k) : expr k
-    | LetIn (name_hint: string) {tx: type} (ex: expr tx) {tC: type} (eC: var tx -> expr tC) : expr tC
-    | SetField {C} {te} (e: expr (typeWithHole.plug C te)) (v: expr te): expr (typeWithHole.plug C te)
-    | GetField {C} {t} (e: expr (typeWithHole.plug C t)) : expr t.
-
+    | Cond {t} (_ : expr Bool) (a b : expr t) : expr t
+    | Let (name_hint: string) {tx: type} (ex: expr tx) {tC: type} (eC: var tx -> expr tC) : expr tC
+    | Get {C : typeWithHole} {t} (r : expr (C t)) (i : expr C) : expr t
+    | Upd {C : typeWithHole} {t} (r : expr (C t)) (i : expr C)
+       (v : var t -> expr t) : expr (typeWithHole.plug C t).
   End WithSubstitutionType.
-
   Arguments expr : clear implicits.
 
-  Fixpoint interp {t} (e: expr type_denote t) : type_denote t :=
-    match e in expr _ t return type_denote t with
-    | Var _ x => x 
-    | Const _ c => c
-    | Unop _ _ op e1 => unop.interp op (interp e1)
-    | Binop _ _ _ op e1 e2 => binop.interp op (interp e1) (interp e2)
-    | ITE _ cond tbranch fbranch => 
-        if interp cond then interp tbranch else interp fbranch
-    | LetIn _ _ ex _ eC => let x := interp ex in interp (eC x)
-    | SetField _ _ e v => 
-        typeWithHole.fieldUpdate (interp e) (interp v)
-    | GetField _ _ e =>
-        typeWithHole.getField (interp e)  
+  Fixpoint interp {t} (e: expr type.interp t) : type.interp t :=
+    match e in expr _ t return type.interp t with
+    | Var x => x
+    | Const c => c
+    | Unop op e1 => unop.interp op (interp e1)
+    | Binop op e1 e2 => binop.interp op (interp e1) (interp e2)
+    | Cond e a b => if interp e then interp a else interp b
+    | Let _ ex eC => let x := interp ex in interp (eC x)
+    | Get r i => typeWithHole.getField (interp r) (interp i)
+    | Upd r i fv => typeWithHole.updField (interp r) (interp i) (fun v => interp (fv v))
     end.
 
 End expr.
@@ -175,50 +244,35 @@ Module action.
 
     Import expr.
     Inductive action : type -> type -> Type :=
-    | GetSt {env_t} : action env_t env_t
-    | PutSt {env_t} (st: expr var env_t) : action env_t Unit
-    (* | LetNonDet (name_hint: string) {tx: type} {tC: type} (eC: var tx -> action tC) : action tC *)
-    (* | LetInput {env_t} (name_hint: string) {tx: type} {tC: type} (eC: var tx -> action env_t tC) : action env_t tC *)
-    | LetAction {env_t} (name_hint: string) {tx: type} (x: action env_t tx) {tC: type} (eC: var tx -> action env_t tC) : action env_t tC
-    | StateUpdate {C} {te} (v: expr var te) : action (typeWithHole.plug C te) Unit
-    (* | Output {env_t} {te: type} (e: expr var te) : action env_t Unit *)
-    | MethodCall {C} {te} {tret} {targ} (arg: expr var targ) (fn: var targ -> @action te tret) : action (typeWithHole.plug C te) tret
-    | Return {env_t} {t: type} (e: expr var t) : action env_t t
+    | Ret {s t} (e : var s -> expr var t) : action s t
+    | Put {s} (e : var s -> expr var s) : action s Unit
+    | Bind {s} (name_hint : string) {tx} (a : action s tx) {t}
+      (aC : var tx -> action s t) : action s t
+    | Cond {s t} (_ : var s -> expr var Bool) (a b : action s t) : action s t
+    | Upd {C : typeWithHole} {t r} (s := C t) (i : var s -> expr var C) (fv : var s -> action t r) : action s r
     .
   End WithSubstitutionType.
 
   Arguments action : clear implicits.
 
   Section WithState.
-    Fixpoint interp {env_t: type} {t} (e: action type_denote env_t t) (env: type_denote env_t) 
-      : type_denote t * type_denote env_t :=
-      match e in action _ env_t' t' 
-              return type_denote env_t' -> (type_denote t' * type_denote env_t')  with
-      | GetSt _ => fun env => (env, env)
-      | PutSt _ st => fun env => (unit_value, expr.interp st)
-      (* (* | LetNonDet _ tx tC eC => *) *)
-      (* (*     fun post => forall x, interp (eC x) env ios post *) *)
-      | LetAction _ _ tx x tC eC =>
-          fun env =>
-          let '(rX, env') := interp x env in
-          interp (eC rX) env'
-      (* | LetInput _ _ tx tC eC => *)
-      (*     fun env post => forall x, *)
-      (*     let io : io_t := IOInput (existT _ x) in *)
-      (*     interp (eC x) env (io::ios) post *)
-      (* | Output _ t te => fun env post => *)
-      (*     let out_val := expr.interp te in *)
-      (*     let io : io_t := IOOutput (existT _ out_val) in *)
-      (*     post (unit_value, env, io::ios) *)
-      | StateUpdate C te v => fun env =>
-          (unit_value, typeWithHole.fieldUpdate env (expr.interp v))
-      | MethodCall C te tret targ arg fn => fun env =>
-          let '(r, env') := interp (fn (expr.interp arg)) (typeWithHole.getField env) in
-          (r, typeWithHole.fieldUpdate env env')
-      | Return _ _ e => fun env => (expr.interp e, env)
-      end env.
+    Fixpoint interp {s t} (e: action type.interp s t) : s -> s * t :=
+      match e in action _ s t return s -> s * t with
+      | Ret e => fun s => (s, expr.interp (e s))
+      | Put e => fun s => let v := expr.interp (e s) in (v, unit_value)
+      | Bind _ a aC => fun s =>
+          let '(s, v) := interp a s in
+          interp (aC v) s
+      | Cond e a b => fun s => if expr.interp (e s) then interp a s else interp b s
+      | Upd i fv => fun s =>
+          let i := expr.interp (i s) in
+          let ms := typeWithHole.getField s i in
+          let (ms, v) := interp (fv s) ms in
+          (typeWithHole.updField s i (fun _ => ms), v)
+      end.
   End WithState.
 End action.
+Notation action := action.action (only parsing).
 
 Module example.
   Section WithSubstitutionType.
@@ -227,16 +281,14 @@ Module example.
     Local Coercion var : type >-> Sortclass.
     Let exprVar {t} := expr.Var (var := var) (tx := t).
 
-    Definition add n (x y : Bits n) : expr var (Bits n) :=
-      expr.Binop binop.Plus (expr.Const x) (expr.Const y). 
+    Definition add {n} (x y : Bits n) : expr var (Bits n) :=
+      expr.Binop binop.Plus (expr.Const x) (expr.Const y).
 
   End WithSubstitutionType.
 
   Lemma add_ok n (x y: Bits n) :
-    expr.interp (add x y) = (x + y)%bv.
-  Proof.
-    reflexivity.
-  Qed.
+    expr.interp (add x y) = Zmod.add x y.
+  Proof. trivial. Qed.
 
   (* TODO: struct example *)
 End example.
@@ -245,64 +297,109 @@ Module notations.
 
 End notations.
 
-(* Circuit:
-   - Cinput/Cregister 
-   - var input -> Expr   
-   - COutput
-   - CBundle 
-   
- *)
 
 Module flat.
   Section WithSubstitutionType.
-    Context {var: type -> Type}.
-    Inductive expr : type -> Type := 
-    | Var {tx: type} (x: var tx) : expr tx
-    | Const {tc: type} (c: type_denote tc) : expr tc
-    | Unop {t1 tR: type} (op: unop t1 tR) (e1: expr t1) : expr tR
-    | Binop {t1 t2 tR: type} (op: binop t1 t2 tR) (e1: expr t1) (e2: expr t2) : expr tR
-    | ITE {k: type} (cond: expr Bool) (tbranch fbranch: expr k) : expr k
-    | GetField {C} {t} (e: expr (typeWithHole.plug C t)) : expr t.
+  Context {var: type -> Type}.
+  (* cases of [expr.expr] without binders *)
+  Inductive expr : type -> Type :=
+  | Var {tx: type} (x: var tx) : expr tx
+  | Const {tc: type} (c: type.interp tc) : expr tc
+  | Unop {t1 tR: type} (op: unop t1 tR) (e1: expr t1) : expr tR
+  | Binop {t1 t2 tR: type} (op: binop t1 t2 tR) (e1: expr t1) (e2: expr t2) : expr tR
+  | Cond {t} (_ : expr Bool) (a b : expr t) : expr t
+  | Get {C : typeWithHole} {t} (r : expr (C t)) (i : expr C) : expr t.
 
-    (* see UnderLets in mit-plv/rewriter *)
-    Inductive underlets (T : Type) :=
-    | LetIn (name_hint: string) {tx: type} (ex: expr tx) (eC: var tx -> underlets T)
-    | LetUpdate {C} {te} (e: expr (typeWithHole.plug C te)) (v: expr te) (eC : var (typeWithHole.plug C te) -> underlets T)
-    | Ret (_ : T).
+  (* cases of [expr.expr] with binders, returning T instead of expr t *)
+  Inductive flat {T : Type} :=
+  | Let (name_hint: string) {tx: type} (ex: expr tx) (eC: var tx -> flat)
+  | Upd {C : typeWithHole} {t} (x: expr (C t)) (i : expr C) (v: expr t) (eC : var (C t) -> flat)
+  | Ret (_ : T).
 
-    Fixpoint compile {env_t: type} {ret: type} (a: action.action var env_t ret) 
-      : (var env_t -> underlets (var env_t * expr ret)).
-      refine
-      match a in (action.action _ env_t' ret') return (var env_t' -> underlets (var env_t' * expr ret')) with
-      | action.GetSt _ => fun env => 
-        Ret (env, Var env)
-      | _ => _ end.
-    Abort.
+  Definition let_ {T} (name_hint: string) {tx: type} (ex: expr tx) : forall (eC: var tx -> flat), @flat T :=
+    match ex with
+    | Var v => fun eC => eC v
+    | ex => fun eC => Let name_hint ex eC
+    end.
+  End WithSubstitutionType.
 
-    (*
-      | action.PutSt _ env' => fun env => 
-          expr.Binop binop.MkPair (@expr.Const _ (Bits 0) unit_value) env'
-      | action.LetAction _ name_hint  _ ax _ cont => fun env => 
-          expr.LetIn name_hint (@compile _ _ ax env) (fun x => 
-          expr.LetIn (name_hint ++ "#env") (expr.Unop unop.Snd (expr.Var x)) (fun env' => 
-          expr.LetIn (name_hint ++ "#ret") (expr.Unop unop.Fst (expr.Var x)) (fun ret => 
-          @compile _ _ (cont ret) env')))                                              
-      | action.StateUpdate C te exp => fun env => 
-          expr.Binop binop.MkPair (@expr.Const _ (Bits 0) unit_value)
-                                  (expr.LetUpdate (expr.Var env) exp)
-      | action.MethodCall C te tret targ arg cont => fun env =>
-          expr.LetIn "TODO_name_hint" arg (fun arg_expr =>
-          expr.LetIn "TODO_field" (expr.GetField (expr.Var env)) (fun sub_env =>
-          expr.LetIn "TODO_subExpr" (@compile _ _ (cont arg_expr) sub_env) (fun sub_env'_and_ret => 
-          let sub_env' := (expr.Unop unop.Snd (expr.Var sub_env'_and_ret)) in
-          let ret := (expr.Unop unop.Fst (expr.Var sub_env'_and_ret)) in 
-          expr.Binop binop.MkPair ret (expr.LetUpdate (expr.Var env) sub_env') 
-          )))
-      | action.Return _ _ exp => fun env => expr.Binop binop.MkPair exp (expr.Var env) 
+  #[global] Arguments expr : clear implicits.
+  #[global] Arguments flat : clear implicits.
+
+  Section WithSubstitutionType.
+  Context {var: type -> Type}.
+  Fixpoint bind {A B} (a : flat var A) (b : A -> flat var B) : flat var B :=
+    match a with
+    | Let x e C => Let x e (fun v => bind (C v) b)
+    | Upd e i v C => Upd e i v (fun v => bind (C v) b)
+    | Ret a => b a
+    end.
+  End WithSubstitutionType.
+End flat.
+Notation flat := flat.flat (only parsing).
+
+Module flatten.
+  Section WithSubstitutionType.
+  Context {var: type -> Type}.
+  Fixpoint expr {t} (e : expr var t) : flat var (flat.expr var t) :=
+    match e in expr _ t return flat var (flat.expr var t) with
+    | expr.Var x => flat.Ret (flat.Var x)
+    | expr.Const c => flat.Ret (flat.Const c)
+    | expr.Unop u e => flat.bind (expr e) (fun v => flat.Ret (flat.Unop u v))
+    | expr.Binop u e1 e2 =>
+      flat.bind (expr e1) (fun v1 =>
+      flat.bind (expr e2) (fun v2 =>
+      flat.Ret (flat.Binop u v1 v2)))
+    | expr.Cond e1 e2 e3 =>
+      flat.bind (expr e1) (fun v1 =>
+      flat.bind (expr e2) (fun v2 =>
+      flat.bind (expr e3) (fun v3 =>
+      flat.Ret (flat.Cond v1 v2 v3))))
+    | expr.Get e1 e2 =>
+      flat.bind (expr e1) (fun v1 =>
+      flat.bind (expr e2) (fun v2 =>
+      flat.Ret (flat.Get v1 v2)))
+    | expr.Let x e C =>
+      flat.bind (expr e) (fun e =>
+      flat.let_ x e (fun v => expr (C v)))
+    | expr.Upd es ei e3 =>
+      flat.bind (expr es) (fun es =>
+      flat.bind (expr ei) (fun ei =>
+      flat.let_ "$eupd" (flat.Get es ei) (fun ef =>
+      flat.bind (expr (e3 ef)) (fun ef =>
+      flat.Upd es ei ef (fun es => flat.Ret (flat.Var es))))))
+    end.
+
+    Fixpoint action {s t} (a : action var s t) : (var s -> flat var (flat.expr var s * flat.expr var t)) :=
+      match a in action _ s t return (var s -> flat var (flat.expr var s * flat.expr var t)) with
+      | action.Ret e => fun s =>
+        flat.bind (expr (e s)) (fun e => flat.Ret (flat.Var s, e))
+      | action.Put e => fun s =>
+        flat.bind (expr (e s)) (fun e =>
+        flat.Ret (e, @flat.Const _ Unit unit_value ))
+      | action.Bind x a aC => fun s =>
+        flat.bind (action a s) (fun '(s', ev) =>
+        flat.let_ x ev (fun v =>
+        action (aC v) s))
+      | action.Upd ei fv => fun s =>
+        flat.bind (expr (ei s)) (fun ei =>
+        flat.let_ "$aupd" (flat.Get (flat.Var s) ei) (fun fs =>
+        flat.bind (action (fv s) fs) (fun '(rs, rv) =>
+        flat.Upd (flat.Var s) ei rs (fun s =>
+        flat.Ret (flat.Var s, rv)))))
+      | action.Cond c a1 a2 => fun s =>
+        flat.bind (action a1 s) (fun '(s1, e1) =>
+        flat.bind (action a2 s) (fun '(s2, e2) =>
+        flat.bind (expr (c s)) (fun c =>
+        flat.Let "$acs" (flat.Cond c (s1) (s2)) (fun s =>
+        flat.Let "$ace" (flat.Cond c e1 e2) (fun e =>
+        flat.Ret (flat.Var s, flat.Var e))))))
       end.
+  End WithSubstitutionType.
 
+  (*
   Theorem correct:
-    forall env_t ret (a: action.action type_denote env_t ret) (env: env_t),
+    forall env_t ret (a: action.action type.interp env_t ret) (env: env_t),
       expr.interp (compile a env) = action.interp a env.
   Proof.
     (* TODO: Fix proof. *)
@@ -311,10 +408,11 @@ Module flat.
     - intros. case_match. rewrite H. rewrite H0. auto.
   Qed.
      *)
-  End WithSubstitutionType.
-  #[global] Arguments expr : clear implicits.
-  #[global] Arguments underlets : clear implicits.
-End flat.
+End flatten.
+
+From quartz Require VerilogSyntax.
+
+Require Import AdmitAxiom.
 
 Module verilog.
   Import (notations)ListNotations.
@@ -322,76 +420,142 @@ Module verilog.
   Import flat.
   Local Unset Asymmetric Patterns.
   Section WithVerilogIdentifier.
-    Context {VId : Set}.
+    Context {VId : Set} (field_name : string -> VId).
     Context {gensym_state : Type} (gensym : gensym_state -> string -> VId * gensym_state).
     Let var (_ : type) := VId.
 
-    Fixpoint expr {t} (e : expr var t) : @VExpr VId.
-    refine
+    Fixpoint const {t : type} : t -> @VExpr VId :=
+      match t return t -> @VExpr VId with
+      | Bool => fun v => VExprPriLiteral (VIntegralBinary (Some 1) (Z.b2z v))
+      | Bits n => fun v =>
+          VExprPriLiteral (
+          (if Z.ltb n 8 return _->_->VIntegralNumber
+            then VDecimalNumberB else VIntegralHex)
+          (Some n) (Zmod.unsigned v))
+      | _ => fun _ => ltac:(admit)
+      end.
+
+    Fixpoint lvalue (c : typeWithHole) (e : @VExpr VId) : @VExpr VId :=
+      match c with
+      | typeWithHole.HOLE => e
+      | typeWithHole.Struct _ n c _ =>
+        lvalue c (VExprHier e (VExprId (field_name n)))
+      | _ => ltac:(admit)
+      end.
+
+    Definition unop {a b} (u : unop a b) : VUniOp :=
+      match u with
+      | unop.Not => VUniNot
+      end.
+
+    Fixpoint expr {t} (e : expr var t) : @VExpr VId :=
       match e with
       | Var x => VExprId x
-      | ITE c t f => VExprCond (@expr _ c) (@expr _ t) (@expr _ f)
-      | _ => ltac:(admit)
+      | Const c => const c
+      | Cond c t f => VExprCond (@expr _ c) (@expr _ t) (@expr _ f)
+      | Unop u e => VExprUniOp (unop u) (@expr _ e)
+      | Binop _ _ _ => ltac:(admit)
+      | @Get _ c _ e TODO_i => lvalue c (expr e)
       end.
-    Admitted.
 
-    Fixpoint stmt {t} (s : underlets var (flat.expr var t)) (g : gensym_state) : list (@VStatementItem VId).
-    refine
+    Fixpoint stmts {a b} (s : flat var (flat.expr var a * flat.expr var b)) (g : gensym_state) (fs ft : VId) : list (@VStatementItem VId) :=
       match s with
-      | LetIn x ex eC =>
+      | Let x ex eC =>
           let '(x, g) := gensym g x in
           VStatementItemBlockingAssignNormal (VExprId x) (expr ex) ::
-          @stmt _ (eC x) g
-      | _ => ltac:(admit)
+          @stmts _ _ (eC x) g fs ft
+      | @Upd _ _ c _ e TODO_i v eC =>
+          let '(x, g) := gensym g EmptyString in
+          VStatementItemBlockingAssignNormal (VExprId x) (expr e) ::
+          VStatementItemBlockingAssignNormal (lvalue c (VExprId x)) (expr v) ::
+          @stmts _ _ (eC x) g fs ft
+      | Ret (a, b) =>
+          VStatementItemBlockingAssignNormal (VExprId fs) (expr a) ::
+          VStatementItemBlockingAssignNormal (VExprId ft) (expr b) ::
+          nil
       end.
-    Abort.
   End WithVerilogIdentifier.
 End verilog.
 
-Print LoadPath.
+Local Open Scope string_scope.
+Import typeWithHole VerilogSyntax.
+Compute verilog.lvalue id HOLE (VExprId "x").
+Compute verilog.lvalue id (Struct [("aa", Bool)] "bb" (Struct [("a", Bool)] "b" HOLE []) []) (VExprId "x").
 
-Module exampleBlinky.
-  Notation width := 27%N.
-  Section WithSubstitutionType.
-    Context {var: type -> Type}.
+Module fifo1.
+  Import typeWithHole expr action.
+  Definition T := Bits 42.
+  Definition state := type.Struct [("len", Bool); ("data", T)].
+  Definition enq {var} (d : var T) : action var state Unit :=
+    Bind "_unit"
+    (Upd (C:=typeWithHole.Struct [] "len" HOLE [("data", T)])
+         (fun _ => @Const _ Unit unit_value)
+         (fun _ => Put (fun _ => @Const _ Bool true))) (fun _ =>
+    (Upd (C:=typeWithHole.Struct [("len", Bool)] "data" HOLE [])
+         (fun _ => @Const _ Unit unit_value)
+         (fun _ => Put (fun _ => Var d)))).
+  Definition len {var} (s : var state) : expr var Bool :=
+    Get (C:=typeWithHole.Struct [] "len" HOLE [("data", T)])
+      (Var s) (@Const _ Unit unit_value).
+  Definition peek {var} (s : var state) : expr var T :=
+    Get (C:=typeWithHole.Struct [("len", Bool)] "data" HOLE [])
+      (Var s) (@Const _ Unit unit_value).
+  Definition deq {var} : action var state T :=
+    Bind "_unit"
+    (Upd (C:=typeWithHole.Struct [] "len" HOLE [("data", T)])
+         (fun _ => @Const _ Unit unit_value)
+         (fun _ => Put (fun _ => @Const _ Bool false))) (fun _ =>
+    Ret peek).
+End fifo1.
 
-    Definition env_t : type := (Bits width).
-    Import action.
-    Definition blinkyCtr (arg: var (Bits width)) : action var env_t Bool :=
-      LetAction "st" GetSt (fun st =>
-      LetAction "_" (PutSt (expr.Binop binop.Plus 
-                              (expr.Var st) 
-                              (expr.Binop binop.Plus
-                                          (@expr.Const _ (Bits width) (Z_to_bv _ 1))
-                                          (expr.Var arg)
-                              )
-                           )) (fun _ =>
-      Return (expr.Binop (binop.Compare false binop.cGt) 
-                         (expr.Var st) 
-                         (@expr.Const _ (Bits width) (Z_to_bv _ (2^26)%Z))))).
+Require Import DecimalString.
+Definition gensym_st : Type := list string * Z.
+Definition gensym (st : gensym_st) (s : string) : string * gensym_st :=
+  let (st, n) := st in
+  if orb (String.eqb "" s) (List.existsb (String.eqb s) st)
+  then let s := s ++ "$" ++ NilEmpty.string_of_int (Z.to_int n) in (s, (cons s st, n+1))
+  else (s, (cons s st, n)).
+Import action fifo1.
+Local Notation "verilog_stmt:( t ')'" := t (t custom verilog_stmt).
+Local Notation "$ x" := (x) (x constr at level 0, in custom verilog_expr at level 1).
+Compute let d:="d" in let s:="s" in
+  verilog.stmts id gensym (flatten.action (
+  Bind "_ret1" (enq d) (fun _ => (* void action method call *)
+  Bind "_ret2" (deq) (fun _ => (* non-void action method call *)
+  Ret (fun s =>
+    expr.Let "_let" (len s) (fun v => (* value method call *)
+    expr.Var v))
+  ))) s) (nil, 0) "FINAL_STATE" "FINAL_VALUE".
 
-    (*
-    Example blinkyCtrCircuit (arg: var (Bits width)) := circuitSyntax.compile (blinkyCtr arg). 
-    Eval cbv in blinkyCtrCircuit.
-     *)
-
-  End WithSubstitutionType.
-
-  Example blinkyCtrInterp (st: type_denote env_t) (arg: type_denote (Bits width)) 
-    : Some (action.interp (blinkyCtr arg) st) = None.
-  Proof.
-    cbn.
-  Abort.
-
-End exampleBlinky.
+(* ...which in slightly less verbose concrete syntax gives:
+$aupd = s.len
+$0 = s
+$0.len = 1'b1
+_unit = 0'd0
+$aupd$1 = s.data
+$2 = s
+$2.data = d
+_ret1 = 0'd0
+$aupd$3 = s.len
+$4 = s
+$4.len = 1'b0
+_unit$5 = 0'd0
+_ret2 = s.data
+_let = s.len
+FINAL_STATE = s
+FINAL_VALUE = _let
+ *)
 
 (* NEXT STEPS:
    - Verilog
      - Expr -> always_comb verilog blocks
-   - Notations :) --> customEntry fun 
+     - Reference: https://github.com/Cherified/Guru/blob/main/PrettyPrinter/CodePrinter.hs
+   - Notations :) --> customEntry fun
+     - Reference: https://github.com/mit-plv/bedrock2/blob/master/bedrock2/src/bedrock2/NotationsCustomEntry.v#L9
+     - Reference: https://github.com/mit-plv/fiat2/blob/main/fiat2/src/fiat2/Notations.v#L158
+     - Reference: VerilogSyntax.v
    - Pretty Gallina reflection/verification stuffs
      - Reification of lvalues/holes
        - Ltac2 silliness
-   - Test on module+nested module
 *)
 
